src3.0/Vellvm/Dominators/dfs.v
@@ -90,9 +90,14 @@ Proof.
   omega.
 Qed.
 
+Definition stk_takes_succs succs (stk : list Frame) : Prop :=
+List.Forall (fun fr : Frame => 
+             incl (Fr_scs fr) (XATree.children_of_tree succs)) stk.
+
+Hint Unfold stk_takes_succs.
+
 Lemma find_next_visit_in_stk_spec1: forall succs visited (stk : list Frame)
-  (Hp : Forall (fun fr : Frame => 
-                incl (Fr_scs fr) (XATree.children_of_tree succs)) stk)  
+  (Hp : stk_takes_succs succs stk)  
   po (next : l) (stk' : list Frame) po'
   (Hfind : inl (next, stk', po') = find_next_visit_in_stk succs visited po stk),
   Forall 
@@ -137,8 +142,7 @@ Qed.
 Lemma find_next_visit_in_stk_spec3: forall succs visited 
   (Hinc: incl (XATree.parents_of_tree visited) (XATree.children_of_tree succs))
   (stk : list Frame) 
-  (Hp : Forall (fun fr : Frame => 
-                incl (Fr_scs fr) (XATree.children_of_tree succs)) stk)
+  (Hp : stk_takes_succs succs stk)
   (next : l) (stk' : list Frame) po po'
   (Hfind : inl (next, stk', po') =
                    find_next_visit_in_stk succs visited po stk),
@@ -168,8 +172,7 @@ Lemma find_next_visit_in_stk_spec2: forall (succs : ATree.t ls)
   (visited : ATree.t unit)
   (Hinc : incl (XATree.parents_of_tree visited) (XATree.children_of_tree succs))
   (stk : list Frame)
-  (Hp : Forall (fun fr : Frame => 
-                incl (Fr_scs fr) (XATree.children_of_tree succs)) stk)
+  (Hp : stk_takes_succs succs stk)
   (next : l) (stk' : list Frame) po po'
   (Hfind : inl (next, stk', po') = find_next_visit_in_stk succs visited po stk),
   incl (XATree.parents_of_tree (ATree.set next tt visited))
@@ -198,13 +201,11 @@ Qed.
 
 Program Fixpoint dfs_aux (succs: ATree.t ls)
   (visited: ATree.t unit) (po:PostOrder) (stk: list Frame) 
-  (Hp: List.Forall 
-         (fun fr => incl (Fr_scs fr) (XATree.children_of_tree succs)) stk /\
+  (Hp: stk_takes_succs succs stk /\
        incl (XATree.parents_of_tree visited) (XATree.children_of_tree succs))
   {measure 
-    ((fun succs acc => 
-      (length (XATree.children_of_tree succs) - 
-       length (XATree.parents_of_tree visited))%nat) succs visited) }
+     (length (XATree.children_of_tree succs) - 
+      length (XATree.parents_of_tree visited))%nat }
   : PostOrder :=
   match find_next_visit_in_stk succs visited po stk with
   | inr po' => po'
@@ -229,3 +230,182 @@ Next Obligation.
     rewrite XATree.parents_of_empty_tree. 
     intros x Hin. tauto.
 Qed.
+
+Fixpoint stk_isa_path (succs: ATree.t ls) (entry:atom) (stk:list Frame) : Prop :=
+match stk with
+| nil => True
+| mkFrame v _::nil => v = entry
+| mkFrame sc _::(mkFrame n _::_) as stk' => 
+    In sc (succs !!! n) /\ stk_isa_path succs entry stk'
+end.
+
+Definition node_in_stk (a2:atom) (stk:list Frame) : Prop :=
+exists stk1, exists stk3, exists scs2, stk = stk1 ++ mkFrame a2 scs2  :: stk3.
+
+Definition wf_aorder_aux (succs: ATree.t ls) (entry:atom) (po:PostOrder) 
+  (stk: list Frame) : Prop :=
+  forall a1 p1 (Hget: (PO_a2p po) ! a1 = Some p1),
+    (p1 < PO_cnt po)%positive /\
+    forall (Hneq: a1 <> entry), 
+    exists a2, 
+      In a2 ((XATree.make_predecessors succs) !!! a1) /\ 
+      ((exists p2, (PO_a2p po) ! a2 = Some p2 /\ (p2 > p1)%positive) \/
+       node_in_stk a2 stk).
+
+Definition wf_stack (succs: ATree.t ls) (entry:atom) (po:PostOrder) 
+  (stk: list Frame) : Prop :=
+stk_isa_path succs entry stk /\
+stk_takes_succs succs stk /\
+wf_aorder_aux succs entry po stk.
+
+Definition wf_aorder scs (entry:atom) (a2p:ATree.t positive) : Prop :=
+  forall a1 (Hneq: a1 <> entry) p1 (Hget: a2p ! a1 = Some p1),
+  exists a2, exists p2,
+    In a2 ((XATree.make_predecessors scs) !!! a1) /\ 
+    a2p ! a2 = Some p2 /\ (p2 > p1)%positive.
+
+Definition dfs_aux_wf_stack_prop (n:nat) : Prop := forall (succs: ATree.t ls) 
+  (visited: ATree.t unit) 
+  (Heq: n = (length (XATree.children_of_tree succs) - 
+             length (XATree.parents_of_tree visited))%nat)
+  entry (po1:PostOrder) (stk: list Frame) 
+  (Hp: stk_takes_succs succs stk /\
+       incl (XATree.parents_of_tree visited) (XATree.children_of_tree succs))
+  po2 (Hdsf: dfs_aux succs visited po1 stk Hp = po2)
+  (Hwf: wf_stack succs entry po1 stk),
+  wf_aorder succs entry (PO_a2p po2).
+
+Lemma dfs_aux_wf_stack_aux: forall n, dfs_aux_wf_stack_prop n.
+Admitted.
+
+Lemma dfs_aux_wf_stack: forall (succs: ATree.t ls) entry
+  (visited: ATree.t unit) (po1:PostOrder) (stk: list Frame) 
+  (Hp: stk_takes_succs succs stk /\
+       incl (XATree.parents_of_tree visited) (XATree.children_of_tree succs))
+  po2 (Hdsf: dfs_aux succs visited po1 stk Hp = po2)
+  (Hwf: wf_stack succs entry po1 stk),
+  wf_aorder succs entry (PO_a2p po2).
+Proof.
+  intros.
+  assert (J:=@dfs_aux_wf_stack_aux 
+                (length (XATree.children_of_tree succs) - 
+                 length (XATree.parents_of_tree visited))%nat).
+  unfold dfs_aux_wf_stack_prop in J.
+  eauto.
+Qed.
+
+Lemma dfs_wf_order: forall scs entry pinit po (Hdfs: dfs scs entry pinit = po),
+  wf_aorder scs entry (PO_a2p po).
+Proof.
+  unfold dfs. intros.
+  apply dfs_aux_wf_stack with (entry:=entry) in Hdfs; auto.
+  split. constructor; auto.
+  split. constructor; simpl; auto.
+          apply XATree.children_in_children_of_tree.
+    intros a1 p1 Hget.   
+    rewrite ATree.gempty in Hget. congruence.
+Qed.
+
+Definition wf_porder scs (entry:positive): Prop :=
+ forall n (Hneq: n <> entry),
+   exists p, In p ((XPTree.make_predecessors scs) ??? n) /\ 
+   (p > n)%positive.
+
+Lemma asuccs_psuccs_pres_order: forall ascs pscs aentry pentry a2p
+  (Htrans: asuccs_psuccs a2p ascs = pscs) (Hwf: wf_aorder ascs aentry a2p)
+  (Hentry: a2p ! aentry = Some pentry),
+  wf_porder pscs pentry.
+Admitted.
+ 
+(*
+Program Fixpoint dfs_aux' (succs: ATree.t ls) (todo: ls) 
+  {measure (length (XATree.children_of_tree succs))%nat }
+  : unit :=
+  match todo with
+  | nil => tt
+  | next::todo' => 
+      match succs!!!next with
+      | sc::scc' => dfs_aux' (ATree.set next scc' succs) (sc::todo'++[next])
+      | nil => dfs_aux' succs todo'
+      end
+  end.
+Next Obligation.
+  admit.
+Qed.
+Next Obligation.
+  admit.
+Qed.
+Next Obligation.
+  admit.
+Qed.
+
+Definition dfs_aux_wf_stack_prop (n:nat) : Prop := forall (succs: ATree.t ls) 
+  (visited: ATree.t unit) 
+  (Hp: incl (XATree.parents_of_tree visited) (XATree.children_of_tree succs))
+  (Heq: n = (length (XATree.children_of_tree succs) - 
+             length (XATree.parents_of_tree visited))%nat)
+  todo
+  (Hdsf: dfs_aux' succs visited todo Hp = tt), True.
+
+Ltac unfold_dfs_aux' :=
+match goal with
+| |- appcontext [dfs_aux' ?arg] =>
+   unfold dfs_aux'; unfold dfs_aux'_func;
+   Program.Wf.WfExtensionality.unfold_sub dfs_aux' arg;
+   repeat Program.Wf.fold_sub dfs_aux'_func
+(*;
+   repeat fold_dfs_aux
+*)
+end.
+
+Require Import Program.Wf.
+
+Lemma dfs_aux_wf_stack_aux: forall n, dfs_aux_wf_stack_prop n.
+Proof.
+  induction n.
+admit.
+
+    unfold dfs_aux_wf_stack_prop.
+    intros until todo.
+unfold_dfs_aux'.
+simpl.
+
+destruct todo. auto.
+destruct (visited ! l0).
+destruct R.
+
+fold_sub dfs_aux'_func.
+
+match goal with
+| |- appcontext [dfs_aux' ?arg] =>
+   unfold dfs_aux'; unfold dfs_aux'_func;
+   Program.Wf.WfExtensionality.unfold_sub dfs_aux' arg
+(*;
+   repeat Program.Wf.fold_sub dfs_aux_func;
+   repeat fold_dfs_aux
+*)
+end.
+    simpl.
+
+ match goal with
+  | |- appcontext C[Fix_sub _ _ _ _ _ ?arg] =>
+       let app := context C [dfs_aux'_func arg] in
+       change app
+  end.
+
+match goal with
+| |- context [dfs_aux_func (existT _ ?a (existT _ _ (existT _ ?b _)))] => 
+     fold (dfs_aux a)
+end.
+
+
+   unfold dfs_aux.
+   unfold dfs_aux_func.
+   WfExtensionality.unfold_sub dfs_aux arg.
+
+
+
+
+    unfold_dfs_aux.
+
+*)
