src3.0/Vellvm/Dominators/push_iter.v
@@ -6,6 +6,7 @@ Require Import infrastructure_props.
 Require Import Metatheory.
 Require Import Program.Tactics.
 Require Import dom_libs.
+Require Import dfs.
 
 Module Weak_Succ_Dataflow_Solver (NS: PNODE_SET) (L: LATTICEELT).
 
@@ -103,30 +104,22 @@ End Kildall.
 
 End Weak_Succ_Dataflow_Solver.
 
-Module LDoms := Doms (MergeGt).
-Module DomDS := Weak_Succ_Dataflow_Solver (PNodeSetMin) (LDoms).
-
-Definition transfer (n:positive) (input: LDoms.t) : LDoms.t :=
-match input with
-| None => None
-| Some ps => Some (n::ps)
-end.
+Module LDoms := Doms (MergeLt).
+Module DomDS := Weak_Succ_Dataflow_Solver (PNodeSetMax) (LDoms).
 
 Require analysis.
 Require Import infrastructure.
 Import LLVMsyntax.
 
-Parameter bfs: ATree.t ls -> l -> positive -> ATree.t positive.
-
 Definition dom_analyze (f: fdef) : PMap.t LDoms.t :=
   let asuccs := analysis.successors f in
   match LLVMinfra.getEntryBlock f with
   | Some (block_intro le _ _ _) =>
-      let a2p := bfs asuccs le 1%positive in
+      let '(mkPO _ a2p) := dfs asuccs le 1%positive in
       let psuccs := asuccs_psuccs a2p asuccs in
       match ATree.get le a2p with
       | Some pe => 
-        match DomDS.fixpoint psuccs transfer ((pe, LDoms.top) :: nil) with
+        match DomDS.fixpoint psuccs LDoms.transfer ((pe, LDoms.top) :: nil) with
         | None => (PMap.set pe LDoms.top (PMap.init LDoms.bot))
         | Some res => res
         end
@@ -137,22 +130,339 @@ Definition dom_analyze (f: fdef) : PMap.t LDoms.t :=
 
 Module DomMap := LATTICEELT_MAP (LDoms).
 
-Section Mono.
+Lemma propagate_succ_list_st_in_aux: forall out sc st2 scs st1 (Hnotin: ~ In sc scs)
+  (Heq: (DomDS.st_in st1) ?? sc = (DomDS.st_in st2) ?? sc),
+  (DomDS.st_in (DomDS.propagate_succ_list st1 out scs)) ?? sc = 
+    (DomDS.st_in st2) ?? sc.
+Proof.
+  induction scs as [|sc' scs' IHscs']; simpl; intros; auto.
+    rewrite IHscs'; auto.
+    unfold DomDS.propagate_succ.
+    destruct_if; simpl.
+      rewrite PMap.gso; auto.
+Qed.
 
-Lemma ge_lub_left: forall dmap x y, 
-  LDoms.ge (LDoms.lub (dmap??x) (transfer y (dmap??y))) (dmap??x).
+Lemma propagate_succ_list_st_in: forall out sc scs st (Hnotin: ~ In sc scs),
+  (DomDS.st_in (DomDS.propagate_succ_list st out scs)) ?? sc = 
+    (DomDS.st_in st) ?? sc.
+Proof. 
+  intros. apply propagate_succ_list_st_in_aux; auto.
+Qed.
+
+Lemma propagate_succ_list_st_wrk: forall out scs st,
+  PositiveSet.Subset (DomDS.st_wrk st)
+    (DomDS.st_wrk (DomDS.propagate_succ_list st out scs)).
+Proof.
+  induction scs; simpl; intros.
+    intro x; auto.
+    intros x Hin.
+    apply IHscs.
+    unfold DomDS.propagate_succ.
+    destruct_if; simpl.
+      apply PositiveSet.add_2; auto.
+Qed.
+
+Lemma propagate_succ_bot_inv: forall st out sc n
+  (Hnone: (DomDS.st_in (DomDS.propagate_succ st out sc)) ?? n = None),
+  (DomDS.st_in st) ?? n = None.
+Proof.
+  unfold DomDS.propagate_succ.
+  intros.
+  destruct_if; auto.
+    destruct (positive_eq_dec sc n); subst.
+      rewrite PMap.gss in H0.
+      rewrite PMap.gss.
+      rewrite H0.
+      apply LDoms.lub_bot_inv in H0. tauto.
+
+      rewrite PMap.gso in H0; auto.
+      rewrite PMap.gso; auto.
+Qed.
+
+Lemma propagate_succ_nonbot_inv: forall n sc st out 
+  (Hacc: (DomDS.st_in st) ?? n <> None),
+  (DomDS.st_in (DomDS.propagate_succ st out sc)) ?? n <> None.
 Proof.
   intros.
-  unfold transfer.
-  caseEq (dmap ?? y).
-    intros Ysdms Hgety.
-    caseEq (dmap ?? x); simpl; auto.
-      intros Xsdms Hgetx.
-      simpl. apply LDoms.merge_is_tail_of_left.
-  
-    intros Hgety.
-    caseEq (dmap ?? x); simpl; auto with coqlib.
+  intro J.
+  apply propagate_succ_bot_inv in J. auto.
 Qed.
+
+Lemma propagate_succ_list_nonbot_inv: forall n scs st out 
+  (Hacc: (DomDS.st_in st) ?? n <> None),
+  (DomDS.st_in (DomDS.propagate_succ_list st out scs)) ?? n <> None.
+Proof.
+  induction scs as [|sc' scs' IHscs']; simpl; intros;
+    eauto using propagate_succ_nonbot_inv.
+Qed.
+
+Lemma propagate_succ_nonbot: forall (sc : positive) (st : DomDS.state)
+  (out : option (list positive)) (Hnonbot : out <> None),
+  (DomDS.st_in (DomDS.propagate_succ st out sc)) ?? sc <> None.
+Proof.
+  intros.
+  unfold DomDS.propagate_succ.
+  destruct_if; simpl.
+    symmetry in HeqR.
+    apply LDoms.beq_correct in HeqR.
+    apply LDoms.Leq_nonbot_inv_r in HeqR; auto.
+    apply LDoms.lub_nonbot_spec; auto.
+   
+    rewrite PMap.gss.
+    apply LDoms.lub_nonbot_spec; auto.
+Qed.
+
+Lemma propagate_succ_list_nonbot_aux: forall sc scs scs2 scs1 st out
+  (Hnonbot: out <> None) (Hin: In sc scs2) (Heq: scs = scs1 ++ scs2)
+  (Hacc: forall a, In a scs1 -> (DomDS.st_in st) ?? a <> None),
+  (DomDS.st_in (DomDS.propagate_succ_list st out scs2)) ?? sc <> None.
+Proof.
+  induction scs2 as [|sc2' scs2' IHscs2']; simpl; intros.
+    tauto.
+    
+    destruct Hin as [Hin | Hin]; subst. 
+      apply propagate_succ_list_nonbot_inv.
+        apply propagate_succ_nonbot; auto.
+
+      apply IHscs2' with (scs2:=scs1++[sc2']); auto.
+        simpl_env. auto.
+
+        intros a Hina.     
+        destruct (positive_eq_dec sc2' a); subst.
+          apply propagate_succ_nonbot; auto.
+
+          apply propagate_succ_nonbot_inv.
+          destruct_in Hina; auto.
+          simpl in Hina.
+          destruct Hina as [Hina | Hina]; try tauto.
+Qed.
+
+Lemma propagate_succ_list_nonbot: forall sc scs st out
+  (Hnonbot: out <> None) (Hin: In sc scs),
+  (DomDS.st_in (DomDS.propagate_succ_list st out scs)) ?? sc <> None.
+Proof.
+  intros. apply propagate_succ_list_nonbot_aux with (scs:=scs)(scs1:=nil); auto.
+Qed.
+
+Module WorklistProps. Section WorklistProps.
+
+Variable successors: PTree.t (list positive).
+Definition in_cfg := XPTree.in_cfg successors.
+
+Definition wf_state (st: DomDS.state) : Prop :=
+ forall n (Hinwrk: PNodeSetMax.In n st.(DomDS.st_wrk)), in_cfg n.
+
+Lemma wf_state_pick_in_cfg: forall st (WF : wf_state st) n rem
+  (Hpick : Some (n, rem) = PNodeSetMax.pick (DomDS.st_wrk st)),
+  in_cfg n.
+Proof.
+  intros.
+  symmetry_ctx.
+  apply PNodeSetMax.pick_in in Hpick.
+  apply WF in Hpick; auto.
+Qed.
+
+Lemma propagate_succ_list_wf_state_aux: forall (p : PositiveSet.elt) 
+  out scs (st : DomDS.state) (Hwf : wf_state st)
+  (Hinscs: forall sc, In sc scs -> In sc successors ??? p),
+  wf_state (DomDS.propagate_succ_list st out scs).
+Proof.
+  induction scs; simpl; intros; auto.
+    apply IHscs; auto.
+      unfold DomDS.propagate_succ.
+      destruct_if; auto.
+        intros n Hinwrk. simpl in *.
+        destruct (positive_eq_dec n a); subst.
+          eapply XPTree.in_succ__in_cfg; eauto.
+          apply PositiveSet.add_3 in Hinwrk; auto.
+Qed.
+
+Lemma propagate_succ_list_wf_state: forall st (Hwf: wf_state st) rem p 
+  (Hpick: PNodeSetMax.pick (DomDS.st_wrk st) = Some (p, rem)),
+  wf_state 
+    (DomDS.propagate_succ_list 
+      {| DomDS.st_in := DomDS.st_in st; DomDS.st_wrk := rem |}
+      (LDoms.transfer p (DomDS.st_in st) ?? p) successors ??? p).
+Proof.
+  intros.
+  assert 
+    (wf_state {| DomDS.st_in := DomDS.st_in st; DomDS.st_wrk := rem |}) 
+    as Hwf'.
+    intros n Hin. simpl in *.
+    apply PNodeSetMax.pick_some with (n':=n) in Hpick.
+    apply Hwf. tauto.
+  apply PNodeSetMax.pick_in in Hpick.
+  apply Hwf in Hpick.
+  eapply propagate_succ_list_wf_state_aux; eauto.
+Qed.
+
+Lemma in_parents_of_tree__in_initial: forall p
+  (Hin : In p (XPTree.parents_of_tree successors)),
+  PNodeSetMax.In p (PNodeSetMax.initial successors).
+Proof.
+  intros.
+  apply XPTree.parents_of_tree__in_successors in Hin.
+  destruct_conjs.
+  eapply PNodeSetMax.initial_spec; eauto.
+Qed.
+
+Variable entrypoint: positive.
+Definition entrypoints := (entrypoint, LDoms.top) :: nil.
+
+Lemma entrypoints_wf_state:
+  wf_state (DomDS.mkstate (DomDS.start_state_in entrypoints) 
+                          (PNodeSetMax.initial successors)).
+Proof.
+  intros x Hin.
+  simpl in *.
+  apply PNodeSetMax.initial_spec' in Hin.
+  apply XPTree.parents_of_tree__in_successors in Hin.
+  apply XPTree.in_parents_of_tree__in_cfg; auto.
+Qed.
+
+End WorklistProps. End WorklistProps.
+
+Ltac fill_holes_in_ctx :=
+repeat match goal with
+| H: match ?e with
+     | Some _ => _
+     | None => _
+     end |- _ =>
+  match goal with
+  | H1: _ = e |- _ => rewrite <- H1 in H
+  | H1: e = _ |- _ => rewrite H1 in H
+  end
+end.
+
+Module InitOrder. Section InitOrder.
+
+Variable successors: PTree.t (list positive).
+Variable entrypoint: positive.
+Definition predecessors := XPTree.make_predecessors successors.
+Definition in_cfg := XPTree.in_cfg successors.
+
+Definition wf_state (st: DomDS.state) : Prop :=
+forall n (Hincfg: in_cfg n),
+  match (st.(DomDS.st_in)) ?? n with
+  | None => 
+      exists p, 
+        In p (predecessors ??? n) /\ (p > n)%positive /\ 
+        PNodeSetMax.In p st.(DomDS.st_wrk)
+  | Some _ => True
+  end.
+
+Lemma max_of_worklist_isnt_bot: forall st (Hwf: wf_state st) n rem
+  (Hinprt: WorklistProps.wf_state successors st)
+  (Hpick: PNodeSetMax.pick (DomDS.st_wrk st) = Some (n, rem)),
+  (st.(DomDS.st_in)) ?? n <> None.
+Proof.
+  intros.
+  assert (Hin:=Hpick).
+  apply PNodeSetMax.pick_in in Hin.
+  apply PNodeSetMax.pick_max in Hpick.
+  apply Hinprt in Hin. 
+  apply Hwf in Hin.
+  intro Hget.
+  rewrite Hget in Hin.
+  destruct_conjs.
+  eapply PositiveSet.max_elt_2 in Hpick; eauto.
+  apply Hpick. apply ZC1; auto.
+Qed.
+
+Lemma propagate_succ_list_wf_state: forall st (Hwf: wf_state st) 
+  (Hinprt: WorklistProps.wf_state successors st) rem p 
+  (Hpick: PNodeSetMax.pick (DomDS.st_wrk st) = Some (p, rem)),
+  wf_state 
+    (DomDS.propagate_succ_list 
+      {| DomDS.st_in := DomDS.st_in st; DomDS.st_wrk := rem |}
+      (LDoms.transfer p (DomDS.st_in st) ?? p) successors ??? p).
+Proof.
+  intros.
+  assert (Hnonbot:=Hpick).
+  apply max_of_worklist_isnt_bot in Hnonbot; auto.
+  apply LDoms.transfer_nonbot with (p:=p) in Hnonbot.
+  intros n Hincfg.
+  match goal with
+  | |- match ?e with
+       | Some _ => _
+       | None => _
+       end => remember e as R; destruct R; auto; symmetry in HeqR
+  end.
+  destruct (In_dec positive_eq_dec n (successors ??? p)) as [Hin | Hnotin].
+    contradict HeqR.
+    eapply propagate_succ_list_nonbot; eauto.
+
+    rewrite propagate_succ_list_st_in in HeqR; auto.
+    apply Hwf in Hincfg. simpl in HeqR.
+    fill_holes_in_ctx.
+    destruct Hincfg as [p' [J1 [J2 J3]]].
+    destruct (positive_eq_dec p p'); subst.
+      apply XPTree.make_predecessors_correct' in J1. 
+      tauto.
+
+      exists p'.
+      repeat split; auto.
+        apply propagate_succ_list_st_wrk. 
+        simpl.
+        apply PNodeSetMax.pick_remove in Hpick. subst.
+        apply PositiveSet.remove_2; auto.
+Qed.
+
+Lemma pick_gt_bot_successors: forall st 
+  (Hinprt: WorklistProps.wf_state successors st)
+  (Hwf: wf_state st) p rem
+  (Hpick: PNodeSetMax.pick (DomDS.st_wrk st) = Some (p, rem)),
+  forall sc (Hinscs: In sc (successors ??? p)) 
+    (Hbot: (DomDS.st_in st) ?? sc = None),
+    (p > sc)%positive.
+Proof.
+  intros.
+  assert (Hnonbot:=Hpick).
+  eapply max_of_worklist_isnt_bot in Hnonbot; eauto.
+  destruct (positive_eq_dec p sc); subst.
+    congruence.
+
+    assert (in_cfg sc) as Hincfg.
+      apply PNodeSetMax.pick_in in Hpick. 
+      apply Hinprt in Hpick.
+      eapply XPTree.in_succ__in_cfg; eauto.
+    apply Hwf in Hincfg.
+    rewrite Hbot in Hincfg.
+    destruct_conjs.
+    apply PNodeSetMax.pick_max in Hpick.
+    eapply PositiveSet.max_elt_2 in Hpick; eauto.
+      apply Pnlt__Pgt_Peq in Hpick.
+      destruct Hpick as [Hpick | Hpick]; subst; auto.
+      eapply Pgt_trans; eauto.
+Qed.
+
+Definition entrypoints := (entrypoint, LDoms.top) :: nil.
+
+Lemma entrypoints_wf_state: forall
+  (wf_order: forall n (Hneq: n <> entrypoint),
+    exists p, In p (predecessors ??? n) /\ (p > n)%positive),
+  wf_state (DomDS.mkstate (DomDS.start_state_in entrypoints) 
+                          (PNodeSetMax.initial successors)).
+Proof.
+  intros. 
+  intros n Hincfg; simpl.
+  destruct (positive_eq_dec n entrypoint) as [|n0]; subst.
+    rewrite PMap.gss. 
+    rewrite PMap.gi; simpl; auto.
+
+    rewrite PMap.gso; auto. 
+    rewrite PMap.gi; simpl.
+    apply wf_order in n0; auto.
+    destruct n0 as [p [J1 J2]].
+    exists p.
+    repeat split; auto.
+      apply XPTree.in_pred__in_parents in J1; auto.
+      apply WorklistProps.in_parents_of_tree__in_initial; auto.
+Qed.
+
+End InitOrder. End InitOrder.
+
+Module Mono. Section Mono.
 
 (** ** Monotonicity properties *)
 
@@ -162,12 +472,13 @@ Qed.
 
 Variable successors: PTree.t (list positive).
 Variable entrypoint: positive.
+Definition in_cfg := XPTree.in_cfg successors.
 
 Lemma propagate_succ_incr:
   forall st p n,
   DomMap.in_incr 
     st.(DomDS.st_in) 
-    (DomDS.propagate_succ st (transfer p (st.(DomDS.st_in)??p)) n).(DomDS.st_in).
+    (DomDS.propagate_succ st (LDoms.transfer p (st.(DomDS.st_in)??p)) n).(DomDS.st_in).
 Proof.
   unfold DomMap.in_incr, DomDS.propagate_succ; simpl; intros.
   destruct_if.
@@ -175,26 +486,20 @@ Proof.
 
     simpl. 
     case (positive_eq_dec n n0); intro; subst.
-      rewrite PMap.gss. apply ge_lub_left; auto.
+      rewrite PMap.gss. apply LDoms.ge_lub_left; auto.
       rewrite PMap.gso; auto. apply LDoms.ge_refl. 
 Qed.
-
-Definition in_cfg (n:positive) : Prop :=
-  In n (XPTree.parents_of_tree successors) /\ 
-  In n (XPTree.children_of_tree successors).
 
 Definition wf_doms (dmap: PMap.t LDoms.t) : Prop :=
 forall n (Hincfg: in_cfg n),
   match dmap ?? n with
-  | None => forall n' (Hset: dmap ?? n' <> None), (n < n')%positive
+  | None => True
   | Some sdms =>
-      List.Forall (Pgt n) sdms /\
-      if positive_eq_dec n entrypoint 
-      then sdms = nil else In entrypoint sdms        
+      List.Forall (Plt n) sdms
   end.
 
 Lemma lub_transfer_stable: forall dmap (Hwf: wf_doms dmap) p (Hincfg: in_cfg p),
-  dmap ?? p = LDoms.lub dmap ?? p (transfer p dmap ?? p).
+  dmap ?? p = LDoms.lub dmap ?? p (LDoms.transfer p dmap ?? p).
 Proof.
   intros.
   apply Hwf in Hincfg.
@@ -207,7 +512,7 @@ Lemma propagate_succ_self_stable: forall st n p
   (Hwf: wf_doms (DomDS.st_in st)) (Hincfg: in_cfg p),
   (DomDS.st_in st) ?? p = 
   (DomDS.st_in 
-    (DomDS.propagate_succ st (transfer p (DomDS.st_in st) ?? p) n)) ?? p.
+    (DomDS.propagate_succ st (LDoms.transfer p (DomDS.st_in st) ?? p) n)) ?? p.
 Proof.
   destruct st as [dmap rem]. simpl.
   intros.
@@ -219,79 +524,139 @@ Proof.
 Qed.
 
 Lemma propagate_succ_wf_doms:
-  forall st p n (Hwf: wf_doms st.(DomDS.st_in)),
+  forall st p n 
+  (Hwf: wf_doms st.(DomDS.st_in)) (Hin: in_cfg p)
+  (Horder: (DomDS.st_in st) ?? n = None -> (p > n)%positive),
   wf_doms
-    (DomDS.propagate_succ st (transfer p (st.(DomDS.st_in)??p)) n).(DomDS.st_in).
+    (DomDS.propagate_succ st (LDoms.transfer p (st.(DomDS.st_in)??p)) n).(DomDS.st_in).
 Proof.
   intros.
   unfold DomDS.propagate_succ.
   destruct_if. simpl.
   intros x Hincfg.
   case (positive_eq_dec n x); intro; subst.
-    rewrite PMap.gss. admit.
+    rewrite PMap.gss. 
+    apply Hwf in Hincfg. 
+    assert (J:=LDoms.ge_lub_left (DomDS.st_in st) x p).
+    remember ((DomDS.st_in st) ?? x) as R.
+    destruct R.
+      eapply LDoms.ge_Forall; eauto.
+      
+      remember ((DomDS.st_in st) ?? p) as R.
+      destruct R; auto.
+        simpl.
+        apply Hwf in Hin.
+        fill_holes_in_ctx.
+        constructor.
+          apply ZC1. apply Horder. auto.
+          eapply order_lt_order in Hin; eauto.  
 
     rewrite PMap.gso; auto. 
-    apply Hwf in Hincfg.
-    remember ((DomDS.st_in st) ?? x) as R.
-    destruct R as [ds|]; auto.
-      intros n' Hget.
-      case (positive_eq_dec n n'); intro; subst.
-        rewrite PMap.gss in Hget. admit.
-        rewrite PMap.gso in Hget; auto.
+    apply Hwf in Hincfg; auto.
 Qed.
 
-Lemma propagate_succ_list_incr:
-  forall p (Hincfg: in_cfg p) scs st (Hwf: wf_doms (DomDS.st_in st)),
+Lemma propagate_succ_list_incr_aux:
+  forall p (Hincfg: in_cfg p) scs st (Hwf: wf_doms (DomDS.st_in st))
+  (Horder: forall n (Hin: In n scs) (Hbot: (DomDS.st_in st) ?? n = None),
+             (p > n)%positive),
   DomMap.in_incr 
     st.(DomDS.st_in) 
     (DomDS.propagate_succ_list 
-      st (transfer p (st.(DomDS.st_in)??p)) scs).(DomDS.st_in).
+      st (LDoms.transfer p (st.(DomDS.st_in)??p)) scs).(DomDS.st_in).
 Proof.
   induction scs as [|sc scs]; simpl; intros.
     apply DomMap.in_incr_refl.
   
     apply DomMap.in_incr_trans with 
       (DomDS.propagate_succ 
-        st (transfer p (st.(DomDS.st_in)??p)) sc).(DomDS.st_in).
+        st (LDoms.transfer p (st.(DomDS.st_in)??p)) sc).(DomDS.st_in).
       apply propagate_succ_incr; auto.
 
       rewrite propagate_succ_self_stable at 3; auto.
       apply IHscs; auto using propagate_succ_wf_doms.
+         intros. apply propagate_succ_bot_inv in Hbot. auto.
 Qed.
 
-Lemma propagate_succ_list_wf_doms: forall st (Hwf: wf_doms (DomDS.st_in st))
-  rem p scs,
+Lemma propagate_succ_list_wf_doms_aux: forall 
+  p (Hin: in_cfg p) scs st (Hwf: wf_doms (DomDS.st_in st))
+  (Horder: forall n (Hin: In n scs) (Hbot: (DomDS.st_in st) ?? n = None),
+             (p > n)%positive),
   wf_doms
     (DomDS.st_in
        (DomDS.propagate_succ_list 
-          {| DomDS.st_in := DomDS.st_in st; DomDS.st_wrk := rem |}
-          (transfer p (DomDS.st_in st) ?? p) scs)).
-Admitted.
+          st (LDoms.transfer p (DomDS.st_in st) ?? p) scs)).
+Proof.
+  induction scs as [|sc scs]; simpl; intros; auto.
+    rewrite propagate_succ_self_stable at 2; auto.
+    apply IHscs; auto using propagate_succ_wf_doms.
+       intros. apply propagate_succ_bot_inv in Hbot. auto.
+Qed.
 
-Definition wf_state st : Prop :=
-wf_doms st.(DomDS.st_in) /\
-forall n (Hin: PositiveSet.In n (DomDS.st_wrk st)), in_cfg n.
+Definition wf_state st : Prop := 
+WorklistProps.wf_state successors st /\
+InitOrder.wf_state successors st /\
+wf_doms (st.(DomDS.st_in)).
+
+Hint Unfold wf_state.
+
+Lemma propagate_succ_list_wf_doms: forall (st : DomDS.state)
+  (Hwf : wf_state st)
+  (rem : PositiveSet.t) (p : PositiveSet.elt)
+  (Hpick : PNodeSetMax.pick (DomDS.st_wrk st) = Some (p, rem)),
+  wf_doms
+    (DomDS.st_in 
+      (DomDS.propagate_succ_list
+        {| DomDS.st_in := DomDS.st_in st; DomDS.st_wrk := rem |}
+        (LDoms.transfer p (DomDS.st_in st) ?? p) successors ??? p)).
+Proof.
+  intros.
+  destruct Hwf as [? [? ?]].
+  change st.(DomDS.st_in) with 
+    (DomDS.mkstate st.(DomDS.st_in) rem).(DomDS.st_in).
+  apply propagate_succ_list_wf_doms_aux; auto.
+    eapply WorklistProps.wf_state_pick_in_cfg; eauto.
+    intros. eapply InitOrder.pick_gt_bot_successors in Hpick; eauto.
+Qed.
+
+Lemma propagate_succ_list_incr: forall st (Hwf: wf_state st)
+  (rem : PositiveSet.t) (p : PositiveSet.elt)
+  (Hpick : PNodeSetMax.pick (DomDS.st_wrk st) = Some (p, rem)),
+  DomMap.in_incr 
+    st.(DomDS.st_in) 
+    (DomDS.propagate_succ_list 
+      {| DomDS.st_in := DomDS.st_in st; DomDS.st_wrk := rem |}
+      (LDoms.transfer p (st.(DomDS.st_in)??p))
+      (successors ??? p)).(DomDS.st_in).
+Proof.
+  intros.
+  destruct Hwf as [? [? ?]].
+  change st.(DomDS.st_in) with 
+    (DomDS.mkstate st.(DomDS.st_in) rem).(DomDS.st_in).
+  apply propagate_succ_list_incr_aux; auto.
+    eapply WorklistProps.wf_state_pick_in_cfg; eauto.
+    intros. eapply InitOrder.pick_gt_bot_successors in Hpick; eauto.
+Qed.
 
 Lemma propagate_succ_list_wf_state: forall st (Hwf: wf_state st) rem p 
-  (Hpick: PNodeSetMin.pick (DomDS.st_wrk st) = Some (p, rem)),
+  (Hpick: PNodeSetMax.pick (DomDS.st_wrk st) = Some (p, rem)),
   wf_state 
     (DomDS.propagate_succ_list 
       {| DomDS.st_in := DomDS.st_in st; DomDS.st_wrk := rem |}
-      (transfer p (DomDS.st_in st) ?? p) successors ??? p).
-Admitted.
-
-Lemma wf_state_pick_in_cfg: forall st (WF : wf_state st) n rem
-  (Hpick : Some (n, rem) = PNodeSetMin.pick (DomDS.st_wrk st)),
-  in_cfg n.
-Admitted.
+      (LDoms.transfer p (DomDS.st_in st) ?? p) successors ??? p).
+Proof.
+  intros.
+  destruct Hwf as [Hwf1 [Hwf2 Hwf3]].
+  split. apply WorklistProps.propagate_succ_list_wf_state; auto.
+  split. apply InitOrder.propagate_succ_list_wf_state; auto.
+         apply propagate_succ_list_wf_doms; auto.
+Qed.
 
 Definition entrypoints := (entrypoint, LDoms.top) :: nil.
 
 Definition predecessors := XPTree.make_predecessors successors.
 
-Hypothesis wf_entrypoints:
-  predecessors ??? entrypoint = nil /\
-  forall n (Hcfg: in_cfg n), (n <= entrypoint)%positive.
+Hypothesis wf_order: forall n (Hneq: n <> entrypoint),
+  exists p, In p (predecessors ??? n) /\ (p > n)%positive.
 
 Lemma entrypoints_wf_doms:
   wf_doms (DomDS.start_state_in entrypoints).
@@ -301,41 +666,30 @@ Proof.
   rewrite PMap.gsspec.
   rewrite PMap.gi.
   destruct_if.
-    simpl.
-    split; auto.
-    destruct_if.
-
-    repeat rewrite PMap.gi. simpl.  
-    intros.
-    case (positive_eq_dec entrypoint n'); intro; subst.
-      destruct wf_entrypoints as [_ J].
-      apply J in Hincfg. 
-      apply Ple_lteq in Hincfg.
-      destruct Hincfg; auto.
-        congruence.
-
-      rewrite PMap.gso in Hset; auto.
-      rewrite PMap.gi in Hset.
-      unfold LDoms.bot in Hset.
-      congruence.
+    simpl. auto.
+    repeat rewrite PMap.gi. simpl. auto.
 Qed.
 
 Lemma entrypoints_wf_state:
   wf_state (DomDS.mkstate (DomDS.start_state_in entrypoints) 
-                          (PNodeSetMin.initial successors)).
-Admitted.
+                          (PNodeSetMax.initial successors)).
+Proof.
+  split. apply WorklistProps.entrypoints_wf_state.
+  split. apply InitOrder.entrypoints_wf_state; auto.
+         apply entrypoints_wf_doms.
+Qed.
 
 Lemma wf_state__wf_doms: forall st (Hwf: wf_state st), wf_doms st.(DomDS.st_in).
-Proof. intros. destruct Hwf. auto. Qed.
+Proof. unfold wf_state. tauto. Qed.
 
 Lemma fixpoint_incr:
   forall res
-  (Hfix: DomDS.fixpoint successors transfer entrypoints = Some res),
+  (Hfix: DomDS.fixpoint successors LDoms.transfer entrypoints = Some res),
   DomMap.in_incr (DomDS.start_state_in entrypoints) res /\
     wf_doms res.
 Proof.
   unfold DomDS.fixpoint; intros.
-  eapply (PrimIter.iterate_prop _ _ (DomDS.step successors transfer)
+  eapply (PrimIter.iterate_prop _ _ (DomDS.step successors LDoms.transfer)
     (fun st => 
        DomMap.in_incr (DomDS.start_state_in entrypoints) st.(DomDS.st_in) /\
        wf_state st)
@@ -343,21 +697,24 @@ Proof.
                 wf_doms res)); eauto.
   Case "1".
     intros st [INCR WF]. unfold DomDS.step.
-    remember (PNodeSetMin.pick (DomDS.st_wrk st)) as R.
+    remember (PNodeSetMax.pick (DomDS.st_wrk st)) as R.
     destruct R as [ [n rem] | ]; auto using wf_state__wf_doms.
       split; auto using propagate_succ_list_wf_state.
         apply DomMap.in_incr_trans with st.(DomDS.st_in); auto.
-          change st.(DomDS.st_in) with 
-            (DomDS.mkstate st.(DomDS.st_in) rem).(DomDS.st_in).
-          apply propagate_succ_list_incr; simpl; 
-            eauto using wf_state__wf_doms, wf_state_pick_in_cfg.
+          apply propagate_succ_list_incr; auto.
+
   Case "2".
     split; auto using entrypoints_wf_state.
       apply DomMap.in_incr_refl.
 Qed.
 
-End Mono.
+End Mono. End Mono.
 
+(*
+Hypothesis wf_entrypoints:
+  predecessors ??? entrypoint = nil /\
+  forall n (Hcfg: in_cfg n), (n <= entrypoint)%positive.
+*)
 
 (*
 (** ** Correctness invariant *)
